assert false

fstar/Hacspec.Chacha20.fst
@@ -43,27 +43,29 @@ let chacha20_core (ctr: uint32) (st0: state_t): state_t =
   let state = array_upd st0 12 (array_index st0 12 +. ctr) in
   chacha20_rounds state `array_add (+.)` (state)
 
+let x: FStar.UInt8.t = 2uy
+
 let chacha20_constants_init (): constants_t =
-  let constants: constants_t = array_new_ (secret (pub_u32 0x0)) (4) in
-  let constants = array_upd constants 0 (secret (pub_u32 0x61707865)) in
-  let constants = array_upd constants 1 (secret (pub_u32 0x3320646e)) in
-  let constants = array_upd constants 2 (secret (pub_u32 0x79622d32)) in
-  let constants = array_upd constants 3 (secret (pub_u32 0x6b206574)) in
+  let constants: constants_t = array_new_ (secret 0ul) (4) in
+  let constants = array_upd constants 0 (secret 0x61707865ul) in
+  let constants = array_upd constants 1 (secret 0x3320646eul) in
+  let constants = array_upd constants 2 (secret 0x79622d32ul) in
+  let constants = array_upd constants 3 (secret 0x6b206574ul) in
   constants
 
 let chacha20_init (key: cha_cha_key_t) (iv: cha_cha_iv_t) (ctr: uint32): state_t =
-  let st: state_t = array_new_ (secret (pub_u32 0)) 16    in
+  let st: state_t = array_new_ (secret 0ul) 16    in
   let st = array_update st 0 (chacha20_constants_init ()) in
   let st = array_update st 4 (array_to_le_uint32s key)    in
   let st = array_upd st 12 ctr                            in
            array_update st 13 (array_to_le_uint32s (iv))
 
 let chacha20_key_block (state : state_t) : block_t =
-  let state: state_t = chacha20_core (secret (pub_u32 0)) state in
+  let state: state_t = chacha20_core (secret 0ul) state in
   array_from_seq 64 (array_to_le_bytes state)
 
 let chacha20_key_block0 (key: cha_cha_key_t) (iv: cha_cha_iv_t): block_t =
-  let state: state_t = chacha20_init (key) (iv) (secret (pub_u32 0)) in
+  let state: state_t = chacha20_init (key) (iv) (secret 0ul) in
   chacha20_key_block state
 
 let chacha20_encrypt_block (st0: state_t) (ctr: uint32) (plain: block_t): block_t =
@@ -72,45 +74,50 @@ let chacha20_encrypt_block (st0: state_t) (ctr: uint32) (plain: block_t): block_
   let st : state_t = pl `array_xor (^.)` st in
   array_from_seq 64 (array_to_le_bytes st)
 
-let chacha20_encrypt_last (st0:state_t) (ctr:uint32) (plain : byte_seq {Seq.length plain <= 64})
-  : r: byte_seq { Seq.length r = seq_chunk_len plain 64 0 }
-  = let b: block_t = array_new_ (secret (pub_u8 0x0)) 64 in
+let chacha20_encrypt_last (st0:state_t) (ctr:uint32) (plain: byte_seq {seq_len plain <= 64})
+  : r: byte_seq { seq_len r = seq_chunk_len plain 64 0 }
+  = let b: block_t = array_new_ (secret (pub_u8 0)) 64 in
   let b = array_update b 0 plain in
   let b = chacha20_encrypt_block st0 ctr b in
   array_slice b 0 (seq_len plain)
 
-let chacha20_update (st0:state_t) (m :byte_seq {Seq.length m >= 64}): byte_seq =
+let chacha20_update (st0:state_t) (m :byte_seq {seq_len m >= 64}): byte_seq =
   let blocks_out: seq uint8 = seq_new_ (secret (pub_u8 0x0)) (seq_len m) in
-  let n_blocks: uint_size = seq_num_exact_chunks m (usize 64) in
-  let blocks_out: seq _ =
-    foldi #(lseq uint8 (Seq.length blocks_out)) 0 n_blocks (fun i blocks_out ->
+  let n_blocks: uint_size = seq_num_exact_chunks m 64 in
+  // [n_blocks] is the number of chunks of size [64] in [m]
+  let blocks_out =
+    foldi #(lseq uint8 (seq_len m)) 0 n_blocks (fun i blocks_out ->
+      // here, [i] ranges from [0] to [n_blocks-1], that is, we consider only complete blocks
       let msg_block: seq uint8 = seq_get_exact_chunk m 64 i in
       let b: block_t = chacha20_encrypt_block st0 (secret (pub_u32 i)) (array_from_seq 64 msg_block) in
       seq_set_exact_chunk blocks_out 64 i b
     ) blocks_out 
   in
-  let blocks_out : lseq uint8 (Seq.length blocks_out) = blocks_out in
-  let last_block : seq uint8 =
-    seq_get_remainder_chunk m 64
-  in
-  // assert (n_blocks == Seq.length m / 64);
-  // assert (Seq.length last_block <= 64);
-  // assert (Seq.length last_block == 64);
-  // assert (seq_chunk_len blocks_out 64 n_blocks <= Seq.length last_block);
-  // assert (seq_chunk_len blocks_out 64 n_blocks == Seq.length last_block);
-  admitP (seq_chunk_len blocks_out 64 n_blocks == Seq.length last_block);
-  if seq_len (last_block) <> 0 then (
+  // [last_block] is the [seq_num_chunks s 64 - 1]th chunk
+  let last_block: seq uint8 = seq_get_remainder_chunk m 64 in
+  if seq_len last_block <> 0 then (
     let b: seq uint8 = chacha20_encrypt_last st0 (secret (pub_u32 n_blocks)) last_block in
-    // assert (Seq.length b == Seq.length last_block);
-    // admitP (Seq.length b = seq_chunk_len blocks_out 64 n_blocks);
+    // we're updating the [n_blocks]th chunk
+    let seq_seq_chunk_precondition = seq_len b == seq_chunk_len blocks_out 64 n_blocks in
+    if seq_len m = 64 then (
+      assert (seq_num_exact_chunks m 64 == 1);
+      assert (seq_num_chunks m 64 - 1 == 0);
+      assert (~seq_seq_chunk_precondition);
+      ()
+    );
+    admitP (seq_seq_chunk_precondition);
+    if seq_len m = 64 then assert (false);
     seq_set_chunk blocks_out 64 n_blocks b
+    // [seq_num_chunks m 64 - 1] ≠ [n_blocks]
+    // [seq_num_chunks m 64 - 1] ≠ [seq_num_exact_chunks m 64]
+    // but `seq_set_chunk` expects `b` to be of same length as `n_blocks`th chunk
   ) else blocks_out
 
 let chacha20
   (key_58 : cha_cha_key_t)
   (iv_59 : cha_cha_iv_t)
   (ctr_60 : pub_uint32)
-  (m_61 : byte_seq)
+  (m_61 : byte_seq {Seq.length m_61 >= 64})
   : byte_seq =
   let state_62 : state_t =
     chacha20_init (key_58) (iv_59) (secret (ctr_60))
